\(B2\) Assuming that the firm’s objective is maximizing the present value of its profits and there is no final period.

Its optimization problem is:

$$max_{k(t),I(t)}\int_0^\infty e^{-rt} [p(t)f(k(t)) - c(I(t))] , s.t. \tag{7}$$

$$\dot{k(t)} = I(t) - \delta k(t),\tag{-}$$

$$k(0) = \bar{k},\tag{-}$$

where k\(.\) and I\(.\) stand for the capital path and the investment path respectively;

f\(.\) is the production function while c\(.\) is the investment cost function.

**\(a\) Find the F.O.C.**

$$\mathcal{L} = \int_0^\infty e^{-rt}[p(t)f(k(t))-c(I(t))]dt + \int_0^\infty \mu(t)\{[I(t)-\delta k(t)]-\dot{k}(t)\}dt + \lambda(\bar{k}-k(0)) $$

$$\\ = \int_0^\infty \{ e^{-rt}[p(t)f(k(t))-c(I(t))]dt + \mu(t)[I(t)-\delta k(t)dt] \} -\int_0^\infty \mu(t)\dot{k} dt + \lambda(\bar{k}-k(0)) $$

$$\\ =  \int_0^\infty \{ e^{-rt}[p(t)f(k(t))-c(I(t))]dt + \mu (t)[I(t)-\delta k(t)]dt\} + \\ \quad \int_0^\infty \mu(t)k(t)dt + \mu(0)k(0) - \mu(\infty)k(\infty)+ \lambda(\bar{k} - k(0))$$

Hamietonian Function

$$H(k(t),I(t),t,\mu(t)) \\ = e^{-rt}[p(t)f(k(t))-c(I(t))] + \mu(t)[I(t)-\delta k(t)]$$

F.O.C

$$\dfrac{\partial H}{\partial I(t)} = 0 \;\; \Rightarrow \;\; -[e^{-rt}c'(I(t))] + \mu(t) = 0 \;\;\;\;\;\tag{*}$$

$$\dfrac{\partial H}{\partial k(t)} + \dot{\mu} = 0 \;\; \Rightarrow \;\; e^{-rt}p(t)f'(k(t)) - \delta \mu(t) + \dot{\mu} = 0 \;\;\;\tag{**}$$

$$\bar{k} = k(0) \tag{-}$$

\(b\) Discuss the condition\(s\) on f\(.\) and c\(.\). The condition\(s\) may or may not related to the necessary and/or sufficient conditions.

\(c\) Show that, if c\(I\(t\)\) = qI\(t\),

$$p(t)f'(k(t)) = (r + \delta)q. \tag{8}$$

Interpret Equation \(8\).

\(d\) Show that, if c ” \(.\) &gt; 0, the optimal paths are characterized by the following pair 3 of differential equations:

$$\dot{k(t)} = I(t) - \delta k(t), \tag{9}$$

$$\dot{I(t)} =\dfrac{ (r + \delta)c'(I(t)) - p(t)f'(k(t)) }{c '' (I(t)) }. \tag{10}$$

Interpret Equations \(9\)-\(10\).

By   $$(\ast)$$

$$\mu(t) = e^{-rt}c'(I(t)) \;\;\; (\ast\ast\ast)$$

By  $$(\ast\ast)$$

$$\dot{\mu(t)} = -e^{-rt}p(t)f'(k(t)) + \delta \mu(t)$$

Put  $$(\ast\ast\ast)$$ into the above equation

$$\dot{\mu(t)} = -e^{-rt}p(t)f'(k(t)) + \delta [e^{-rt}c'(I(t))]$$

However , if we differentiate \(w.r.t. t\) the equation   $$(\ast\ast\ast)$$  directly

$$\dot{\mu(t)} = e^{-rt}(-r)c'(I(t)) + e^{-rt}c''(I(t))\dot{I(t)}$$

Therefore , eliminating  $$\dot{\mu(t)}$$   and   $$e^{-rt}$$

$$-p(t)f'(k(t)) + \delta c'(I(t)) = (-r)c'(I(t)) + c''(I(t))\dot{I(t)}$$

\(e\) Interpret your results in \(a\)-\(d\) with a Cobb-Douglas production function and a quadratic cost function.

